implement Realloc

lib/MutableMapImpl_wip.i.dfy
@@ -254,157 +254,6 @@ module MutableMap {
           FixedSizeHashMap.ModelI(Underlying), Count, Contents)
     }
 
-    //static function I(self: ResizingHashMap<V>): (contents: map<uint64, V>)
-    //requires self.Inv()
-    //ensures contents == self.Contents
-    //reads self, self.Repr
-    //{
-    //  self.Contents
-    //}
-
-  //   static function MapFromStorage(elements: seq<Item<V>>): (result: map<uint64, V>)
-  //   {
-  //     if |elements| == 0 then
-  //       map[]
-  //     else
-  //       var item := Last(elements);
-  //       var dropLastMap := MapFromStorage(DropLast(elements));
-  //       if item.Entry? then
-  //         dropLastMap[item.key := item.value]
-  //       else
-  //         dropLastMap
-  //   }
-
-  //   lemma CantEquivocateMapFromStorageKey(underlying: FixedSizeHashMap<V>)
-  //     requires underlying.Inv()
-  //     ensures forall slot1, slot2 :: ValidSlot(underlying.Storage.Length, slot1) && ValidSlot(underlying.Storage.Length, slot2) &&
-  //         underlying.Storage[slot1.slot].Entry? && underlying.Storage[slot2.slot].Entry? &&
-  //         underlying.Storage[slot1.slot].key == underlying.Storage[slot2.slot].key ==> slot1 == slot2
-  //   {
-  //     assert underlying.Storage.Length > 0;
-  //     assert ValidSlot(underlying.Storage.Length, Slot(0));
-  //     assert exists slot :: ValidSlot(underlying.Storage.Length, slot);
-  //     forall slot1, slot2 | (
-  //       && ValidSlot(underlying.Storage.Length, slot1) && ValidSlot(underlying.Storage.Length, slot2)
-  //       && underlying.Storage[slot1.slot].Entry? && underlying.Storage[slot2.slot].Entry?
-  //       && underlying.Storage[slot1.slot].key == underlying.Storage[slot2.slot].key)
-  //     ensures slot1 == slot2
-  //     {
-  //       assert underlying.CantEquivocateStorageKey(underlying.Storage[..]);
-  //       if underlying.Storage[slot1.slot].Entry? && underlying.Storage[slot2.slot].Entry? &&
-  //         underlying.Storage[slot1.slot].key == underlying.Storage[slot2.slot].key {
-
-  //         assert underlying.TwoNonEmptyValidSlotsWithSameKey(underlying.Storage[..], slot1, slot2);
-  //         if slot1 != slot2 {
-  //           assert false;
-  //         }
-  //         assert slot1 == slot2;
-  //       } else {
-  //         assert slot1 == slot2;
-  //       }
-  //     }
-  //   }
-
-  //   lemma MapFromStorageProperties(elements: seq<Item<V>>, result: map<uint64, V>)
-  //     requires forall slot1, slot2 :: ValidSlot(|elements|, slot1) && ValidSlot(|elements|, slot2) &&
-  //         elements[slot1.slot].Entry? && elements[slot2.slot].Entry? &&
-  //         elements[slot1.slot].key == elements[slot2.slot].key ==> slot1 == slot2
-  //     requires MapFromStorage(elements) == result
-  //     ensures forall slot :: ValidSlot(|elements|, slot) && elements[slot.slot].Entry? ==>
-  //         && var item := elements[slot.slot];
-  //         && item.key in result && result[item.key] == item.value
-  //     ensures forall key :: key in result ==>
-  //         exists slot :: ValidSlot(|elements|, slot) && elements[slot.slot] == Entry(key, result[key])
-  //     ensures forall key :: key !in result ==>
-  //         forall slot :: ValidSlot(|elements|, slot) && elements[slot.slot].Entry?
-  //             ==> elements[slot.slot].key != key
-  //   {
-  //     if |elements| == 0 {
-  //     } else if Last(elements).Entry? {
-  //       var item := Last(elements);
-  //       assert elements == DropLast(elements) + [Last(elements)];
-  //       var dropLastMap := MapFromStorage(DropLast(elements));
-  //       MapFromStorageProperties(DropLast(elements), dropLastMap);
-
-  //       forall slot | ValidSlot(|elements|, slot) && elements[slot.slot].Entry?
-  //       ensures && var item := elements[slot.slot];
-  //               && item.key in result && result[item.key] == item.value
-  //       {
-  //         var slotItem := elements[slot.slot];
-  //         if item.key == elements[slot.slot].key {
-  //           if slot.slot == |elements| - 1 {
-  //             assert slotItem.key in result && result[slotItem.key] == slotItem.value;
-  //           } else {
-  //             var slot := Slot(|elements| - 1);
-  //             assert ValidSlot(|elements|, slot);
-  //             assert false;
-  //           }
-  //         } else {
-  //           assert slotItem.key in result && result[slotItem.key] == slotItem.value;
-  //         }
-  //       }
-  //       forall key | key in result
-  //       ensures exists slot :: ValidSlot(|elements|, slot) && elements[slot.slot] == Entry(key, result[key])
-  //       {
-  //         if key == item.key {
-  //           var slot := Slot(|elements| - 1);
-  //           assert ValidSlot(|elements|, slot);
-  //           assert elements[slot.slot] == Entry(key, result[key]);
-  //         } else {
-  //           assert exists slot :: ValidSlot(|elements|, slot) && elements[slot.slot] == Entry(key, result[key]);
-  //         }
-  //       }
-  //     } else {
-  //     }
-  //   }
-
-  //   predicate UnderlyingContentsMatchesContents(underlying: FixedSizeHashMap<V>, contents: map<uint64, V>)
-  //     reads this, underlying
-  //   {
-  //     && (forall key :: key in contents ==> key in underlying.Contents && underlying.Contents[key] == Some(contents[key]))
-  //     && (forall key :: key !in contents ==> key !in underlying.Contents || underlying.Contents[key].None?)
-  //   }
-
-  //   predicate UnderlyingInv(underlying: FixedSizeHashMap<V>)
-  //   reads this, this.Repr, underlying, underlying.Repr
-  //   {
-  //     && |Contents| == Count as nat
-  //     && UnderlyingContentsMatchesContents(underlying, Contents)
-  //     && underlying.Inv()
-  //     && MapFromStorage(underlying.Storage[..]) == Contents
-  //   }
-
-  //   lemma UnderlyingInvImpliesMapFromStorageMatchesContents(underlying: FixedSizeHashMap<V>, contents: map<uint64, V>)
-  //     requires UnderlyingContentsMatchesContents(underlying, contents)
-  //     requires underlying.Inv()
-  //     ensures MapFromStorage(underlying.Storage[..]) == contents
-  //   {
-  //     var mapFromStorage := MapFromStorage(underlying.Storage[..]);
-  //     CantEquivocateMapFromStorageKey(underlying);
-  //     MapFromStorageProperties(underlying.Storage[..], mapFromStorage);
-  //     assert MapFromStorage(underlying.Storage[..]) == contents;
-  //   }
-
-  //   predicate ReprInv()
-  //     reads this, this.Repr
-  //   {
-  //     && { this, this.Underlying } <= Repr
-  //     && { this, this.Underlying } + this.Underlying.Repr == Repr
-  //     && this.Underlying.Repr == { this.Underlying, this.Underlying.Storage }
-  //   }
-
-  //   protected predicate Inv()
-  //     ensures Inv() ==> ReprInv() // make ReprInv transparent
-  //     ensures Inv() ==> |Contents| == Count as nat
-  //     reads this, this.Repr
-  //   {
-  //     && ReprInv()
-
-  //     && UnderlyingInv(Underlying)
-  //     && MapFromStorage(Underlying.Storage[..]) == Contents
-  //     && |Contents| == Count as nat
-  //   }
-
     constructor (size: uint64)
       requires 128 <= size
       ensures Inv()
@@ -424,207 +273,24 @@ module MutableMap {
       ghost var c := MutableMapModel.Constructor<V>(size);
     }
 
-  //   constructor FromUnderlying(underlying: FixedSizeHashMap<V>, count: uint64)
-  //     requires 128 <= underlying.Storage.Length
-  //     requires underlying.Inv()
-  //     ensures Underlying == underlying
-  //     ensures Count == count
-  //     ensures Contents == map[]
-  //     ensures fresh(this)
-  //     ensures Repr == { this, this.Underlying } + Underlying.Repr
-  //   {
-  //     Count := count;
-  //     Underlying := underlying;
-  //     Contents := map[];
+    constructor FromUnderlying(underlying: FixedSizeHashMap<V>, count: uint64)
+      requires 128 <= underlying.Storage.Length
+      requires underlying.WF()
+      requires underlying.Inv()
+      ensures Underlying == underlying
+      ensures Count == count
+      ensures Contents == map[]
+      ensures fresh(this)
+      ensures Repr == { this, this.Underlying } + Underlying.Repr
+    {
+      Count := count;
+      Underlying := underlying;
+      Contents := map[];
 
-  //     new;
+      new;
 
-  //     Repr := { this, Underlying } + Underlying.Repr;
-  //   }
-
-  //   method ToArray() returns (result: array<(uint64, V)>)
-  //     requires Inv()
-  //     ensures Contents == old(Contents)
-  //     ensures Count == old(Count)
-  //     ensures Count as nat == |Contents|
-  //     ensures result.Length == Count as nat
-  //     ensures forall i: nat, j: nat :: i < result.Length && j < result.Length && result[i].0 == result[j].0
-  //         ==> i == j
-  //     // ??? ensures Contents == map i | 0 <= i < result.Length :: result[i].0 := result[i].1
-  //     ensures forall i: nat | i < result.Length :: result[i].0 in Contents && Contents[result[i].0] == result[i].1
-  //     ensures forall k | k in Contents :: exists i: nat :: i < result.Length && result[i] == (k, Contents[k])
-  //     ensures Repr == old(Repr)
-  //   {
-  //     assume false; // TODO takes too long to verify right now
-  //     if Count == 0 {
-  //       assert Contents == map[];
-  //       result := new [0 as uint64];
-  //       assert Contents == map i | 0 <= i < result.Length :: result[i].0 := result[i].1;
-  //       return;
-  //     }
-  //     assert Count > 0;
-  //     assert exists i: nat :: i < Underlying.Storage.Length && Underlying.Storage[i].Entry?;
-
-
-  //     var storagePos: uint64 := 0;
-  //     while storagePos < Underlying.Storage.Length as uint64 && !Underlying.Storage[storagePos].Entry?
-  //       invariant 0 <= storagePos as int <= Underlying.Storage.Length
-  //       invariant MapFromStorage(Underlying.Storage[..storagePos]) == map[]
-  //       invariant forall i: nat :: i < storagePos as int ==> !Underlying.Storage[i].Entry?
-  //     {
-  //       assert MapFromStorage(Underlying.Storage[..storagePos]) == map[];
-  //       assert !Underlying.Storage[storagePos].Entry?;
-  //       assert DropLast(Underlying.Storage[..storagePos+1]) == Underlying.Storage[..storagePos];
-  //       assert MapFromStorage(Underlying.Storage[..storagePos+1]) == map[];
-
-  //       // -- increment --
-  //       storagePos := storagePos + 1;
-  //       // ---------------
-  //     }
-
-  //     assert storagePos as int != Underlying.Storage.Length;
-
-  //     ghost var transferredContents := map[];
-  //     assert MapFromStorage(Underlying.Storage[..storagePos]) == transferredContents;
-  //     assert transferredContents.Keys <= Contents.Keys;
-
-  //     assert storagePos as int < Underlying.Storage.Length;
-  //     var firstEntry := Underlying.Storage[storagePos];
-  //     assert Underlying.EntryInSlotMatchesContents(Underlying.Storage[..], Slot(storagePos as int), Underlying.Contents);
-  //     assert firstEntry.key in Contents;
-  //     // -- mutation --
-  //     result := Native.Arrays.newArrayFill(Count, (firstEntry.key, firstEntry.value));
-  //     transferredContents := transferredContents[firstEntry.key := firstEntry.value];
-  //     // --------------
-
-  //     assert DropLast(Underlying.Storage[..storagePos+1]) == Underlying.Storage[..storagePos];
-  //     assert MapFromStorage(Underlying.Storage[..storagePos+1]) == transferredContents;
-  //     assert transferredContents.Keys <= Contents.Keys;
-
-  //     // -- increment --
-  //     storagePos := storagePos + 1;
-  //     // ---------------
-
-  //     // assert transferredContents == map[firstEntry.key := firstEntry.value];
-  //     assert result[0] == (firstEntry.key, firstEntry.value); // observe
-
-  //     assert MapFromStorage(Underlying.Storage[..storagePos]) == transferredContents;
-
-  //     var resultPos: uint64 := 1;
-  //     assert forall k | k in transferredContents :: exists i: nat :: i < resultPos as int && result[i] == (k, transferredContents[k]);
-  //     while storagePos < Underlying.Storage.Length as uint64
-  //       invariant 0 <= storagePos as int <= Underlying.Storage.Length
-  //       invariant result.Length == Count as nat
-  //       invariant resultPos as int == |transferredContents|
-  //       invariant resultPos as int <= result.Length
-  //       invariant transferredContents.Keys <= Contents.Keys
-  //       invariant forall k | k in transferredContents :: transferredContents[k] == Contents[k]
-  //       invariant MapFromStorage(Underlying.Storage[..storagePos]) == transferredContents
-  //       invariant MapFromStorage(Underlying.Storage[..]) == Contents
-  //       invariant forall i: nat | i < resultPos as int :: result[i].0 in transferredContents && transferredContents[result[i].0] == result[i].1
-  //       invariant forall i: nat, j: nat :: i < resultPos as int && j < resultPos as int && result[i].0 == result[j].0 ==> i == j
-  //       invariant forall k | k in transferredContents :: exists i: nat :: i < resultPos as int && result[i] == (k, transferredContents[k])
-  //     {
-  //       var item := Underlying.Storage[storagePos];
-
-  //       if item.Entry? {
-  //         if resultPos > result.Length as uint64 {
-  //           assert |transferredContents| > result.Length;
-  //           assert |transferredContents| > |Contents|;
-  //           assert |transferredContents.Keys| > |Contents.Keys|;
-  //           SetInclusionImpliesSmallerCardinality(transferredContents.Keys, Contents.Keys);
-  //           assert false;
-  //         } else if resultPos == result.Length as uint64 {
-  //           // TODO minimize
-  //           assert |transferredContents| == |Contents|;
-  //           assert |transferredContents.Keys| == |Contents.Keys|;
-  //           SetInclusionAndEqualCardinalityImpliesSetEquality(transferredContents.Keys, Contents.Keys);
-  //           assert transferredContents.Keys == Contents.Keys;
-  //           assert transferredContents == Contents;
-  //           ghost var thisSlot := Slot(storagePos as int);
-  //           assert MapFromStorage(Underlying.Storage[..storagePos]) == MapFromStorage(Underlying.Storage[..]);
-  //           assert Underlying.EntryInSlotMatchesContents(Underlying.Storage[..], thisSlot, Underlying.Contents);
-  //           assert item.key in Underlying.Contents;
-  //           assert item.key in Contents;
-  //           CantEquivocateMapFromStorageKey(Underlying);
-  //           MapFromStorageProperties(Underlying.Storage[..storagePos], Contents);
-  //           ghost var previousSlot :| (
-  //               && ValidSlot(Underlying.Storage.Length, previousSlot)
-  //               && previousSlot.slot < storagePos as int
-  //               && Underlying.FilledWithEntryKey(Underlying.Storage[..], previousSlot, item.key));
-  //           assert Underlying.FilledWithEntryKey(Underlying.Storage[..], thisSlot, item.key);
-  //           assert Underlying.TwoNonEmptyValidSlotsWithSameKey(Underlying.Storage[..], previousSlot, thisSlot);
-  //           assert Underlying.CantEquivocateStorageKey(Underlying.Storage[..]);
-  //           assert Underlying.SameSlot(Underlying.Storage.Length, previousSlot, thisSlot);
-  //           assert false;
-  //         }
-  //         assert resultPos as int < result.Length;
-
-  //         if item.key in transferredContents {
-  //           // TODO minimize
-  //           CantEquivocateMapFromStorageKey(Underlying);
-  //           MapFromStorageProperties(Underlying.Storage[..storagePos], transferredContents);
-  //           ghost var previousSlot :| (
-  //               && ValidSlot(Underlying.Storage.Length, previousSlot)
-  //               && previousSlot.slot < storagePos as int
-  //               && Underlying.FilledWithEntryKey(Underlying.Storage[..], previousSlot, item.key));
-  //           ghost var thisSlot := Slot(storagePos as int);
-  //           assert Underlying.FilledWithEntryKey(Underlying.Storage[..], thisSlot, item.key);
-  //           assert Underlying.TwoNonEmptyValidSlotsWithSameKey(Underlying.Storage[..], previousSlot, thisSlot);
-  //           assert Underlying.CantEquivocateStorageKey(Underlying.Storage[..]);
-  //           assert Underlying.SameSlot(Underlying.Storage.Length, previousSlot, thisSlot);
-  //           assert false;
-  //         }
-  //         assert item.key !in transferredContents;
-
-  //         assert Underlying.EntryInSlotMatchesContents(Underlying.Storage[..], Slot(storagePos as int), Underlying.Contents); // observe
-
-  //         ghost var transferredContentsBefore := transferredContents;
-  //         ghost var resultBefore := result[..];
-
-  //         // -- mutation --
-  //         result[resultPos] := (item.key, item.value);
-  //         transferredContents := transferredContents[item.key := item.value];
-  //         resultPos := resultPos + 1;
-  //         // --------------
-
-  //         forall k | k in transferredContents
-  //         ensures exists i: nat :: i < resultPos as int && result[i] == (k, transferredContents[k])
-  //         {
-  //           if k == item.key {
-  //           } else {
-  //             // TODO minimize
-  //             assert exists i: nat :: i < (resultPos as int - 1) && resultBefore[i] == (k, transferredContentsBefore[k]);
-  //             assert resultBefore[..(resultPos as int - 1)] == result[..(resultPos as int - 1)];
-  //             assert exists i: nat :: i < (resultPos as int - 1) && result[i] == (k, transferredContentsBefore[k]);
-  //             assert exists i: nat :: i < (resultPos as int - 1) && result[i] == (k, transferredContents[k]);
-  //             assert exists i: nat :: i < resultPos as int && result[i] == (k, transferredContents[k]);
-  //           }
-  //         }
-
-  //         assert resultPos as int == |transferredContents|;
-  //       }
-
-  //       assert DropLast(Underlying.Storage[..storagePos+1]) == Underlying.Storage[..storagePos];
-
-  //       // -- increment --
-  //       storagePos := storagePos + 1;
-  //       // ---------------
-
-  //       assert transferredContents.Keys <= Contents.Keys;
-  //       assert forall k | k in transferredContents :: transferredContents[k] == Contents[k];
-  //       assert resultPos as int == |transferredContents|;
-  //     }
-
-  //     assert Underlying.Storage[..storagePos] == Underlying.Storage[..];
-  //     assert Contents == transferredContents;
-
-  //     assert forall i: nat, j: nat :: i < result.Length && j < result.Length && result[i].0 == result[j].0
-  //         ==> i == j;
-  //     assert result.Length == Count as nat;
-  //     assert forall i: nat | i < result.Length :: result[i].0 in Contents && Contents[result[i].0] == result[i].1;
-  //     assert forall k | k in Contents :: exists i: nat :: i < result.Length && result[i] == (k, Contents[k]);
-  //   }
+      Repr := { this, Underlying } + Underlying.Repr;
+    }
 
   //   method ToMap() returns (result: map<uint64, V>)
   //     requires Inv()
@@ -637,175 +303,55 @@ module MutableMap {
   //     result := map i: nat | i < asArray.Length :: asArray[i].0 := asArray[i].1;
   //   }
 
-  //   method Realloc()
-  //     requires Count as nat < 0x10000000000000000 / 8
-  //     requires Inv()
-  //     ensures Inv()
-  //     ensures Contents == old(Contents)
-  //     ensures Underlying.Count as nat < Underlying.Storage.Length - 2
-  //     ensures fresh(Underlying)
-  //     ensures fresh(Underlying.Storage)
-  //     ensures forall r :: r in Repr ==> r in old(Repr) || fresh(r)
-  //     modifies this
-  //   {
-  //     assert |Contents| == Count as nat;
+    method Realloc()
+      requires Count as nat < 0x10000000000000000 / 8
+      requires Inv()
+      ensures Inv()
+      ensures Contents == old(Contents)
+      ensures Underlying.Count as nat < Underlying.Storage.Length - 2
+      ensures fresh(Underlying)
+      ensures fresh(Underlying.Storage)
+      ensures forall r :: r in Repr ==> r in old(Repr) || fresh(r)
+      ensures I() == MutableMapModel.Realloc(old(I()))
+      modifies this
+    {
+      MutableMapModel.reveal_ReallocInternal();    
+      var newSize: uint64 := (128 + Count) * 4;
 
-  //     var newSize: uint64 := (128 + Count) * 4;
-  //     //print "(debug) MutableMap.Realloc: Count ", Count, ", Realloc ", newSize, "\n";
+      var newUnderlying := new FixedSizeHashMap(newSize);
+      var i: uint64 := 0;
 
-  //     var newUnderlying := new FixedSizeHashMap(newSize);
-  //     assert fresh(newUnderlying) && fresh(newUnderlying.Storage);
-  //     
-  //     assert newUnderlying.Storage.Length == newSize as nat;
+      while i < Underlying.Storage.Length as uint64
+      invariant newUnderlying.WF();
+      invariant newUnderlying.Inv();
+      invariant 0 <= i as int <= Underlying.Storage.Length
+      invariant Count as int < newUnderlying.Storage.Length - 1
+      invariant newUnderlying.Contents.Keys <= Contents.Keys
+      invariant Inv()
+      invariant I() == old(I())
+      invariant this.Repr == old(this.Repr)
+      invariant fresh(newUnderlying)
+      invariant fresh(newUnderlying.Storage)
+      invariant MutableMapModel.ReallocIterate(I(), FixedSizeHashMap.ModelI(newUnderlying), i)
+             == MutableMapModel.ReallocIterate(I(), MutableMapModel.ConstructorFromSize(newSize), 0)
+      {
+        var item := Underlying.Storage[i];
+        if item.Entry? {
+          SetInclusionImpliesSmallerCardinality(newUnderlying.Contents.Keys, Contents.Keys);
+          MutableMapModel.LemmaFixedSizeInsertResult(FixedSizeHashMap.ModelI(newUnderlying), item.key, item.value);
+          MutableMapModel.LemmaEntryKeyInContents(I(), i);
 
-  //     assert MapFromStorage(Underlying.Storage[..]) == Contents;
-  //     UnderlyingInvImpliesMapFromStorageMatchesContents(newUnderlying, map[]);
-  //     assert MapFromStorage(newUnderlying.Storage[..]) == map[];
+          var _ := newUnderlying.Insert(item.key, item.value);
+        }
+        i := i + 1;
+      }
 
-  //     var i: uint64 := 0;
-  //     ghost var transferredContents := map[];
-  //     while i < Underlying.Storage.Length as uint64
-  //       invariant i as int <= Underlying.Storage.Length
-  //       invariant newUnderlying.Inv()
-  //       invariant |Contents| == Count as nat
-  //       invariant Contents == old(Contents) // this is necessary because of `modifies this` (?)
-  //       invariant UnderlyingContentsMatchesContents(newUnderlying, transferredContents)
-  //       invariant MapFromStorage(Underlying.Storage[..i]) == transferredContents
-  //       invariant MapFromStorage(Underlying.Storage[..]) == Contents
+      this.Underlying := newUnderlying;
 
-  //       invariant newUnderlying.Count as nat <= i as nat
-  //       invariant Underlying == old(Underlying)
-  //       invariant Underlying.Inv()
-  //       invariant Underlying.Count == old(Underlying.Count)
-  //       invariant Underlying.Storage.Length == old(Underlying.Storage.Length)
-  //       invariant newUnderlying.Storage.Length == newSize as nat
+      this.Repr := { this, Underlying } + Underlying.Repr;
 
-  //       invariant |transferredContents| == newUnderlying.Count as nat
-  //       invariant transferredContents.Keys <= Contents.Keys
-  //       invariant forall key :: key in newUnderlying.Contents ==> exists slot: Slot :: (
-  //           && slot.slot < i as int
-  //           && ValidSlot(Underlying.Storage.Length, slot)
-  //           && Underlying.FilledWithEntryKey(Underlying.Storage[..], slot, key))
-
-  //       invariant fresh(newUnderlying)
-  //       invariant fresh(newUnderlying.Storage)
-  //       decreases Underlying.Storage.Length - i as int
-  //     {
-  //       var item := Underlying.Storage[i];
-  //       assert Underlying.Storage[..i+1] == Underlying.Storage[..i] + [Underlying.Storage[i]];
-
-  //       if item.Entry? {
-  //         assert MapFromStorage(Underlying.Storage[..i]) == transferredContents;
-  //         assert |transferredContents| == newUnderlying.Count as nat;
-
-  //         assert fresh(newUnderlying);
-  //         assert fresh(newUnderlying.Storage);
-  //         if item.key in newUnderlying.Contents {
-  //           var j:uint64 :| (
-  //               && 0 <= j < i
-  //               && ValidSlot(Underlying.Storage.Length, Slot(j as int))
-  //               && Underlying.Storage[Slot(j as int).slot].Entry?
-  //               && Underlying.Storage[Slot(j as int).slot].key == item.key);
-  //           assert ValidSlot(Underlying.Storage.Length, Slot(i as nat));
-  //           assert i != j;
-  //           assert Slot(i as nat) != Slot(j as nat);
-  //           assert Underlying.Storage[Slot(j as nat).slot].key == Underlying.Storage[Slot(i as nat).slot].key;
-  //           CantEquivocateMapFromStorageKey(Underlying);
-  //           assert false;
-  //         }
-  //         assert item.key !in newUnderlying.Contents;
-
-  //         assert transferredContents.Keys <= Contents.Keys;
-  //         SetInclusionImpliesSmallerCardinality(transferredContents.Keys, Contents.Keys);
-  //         assert |transferredContents.Keys| <= |Contents.Keys|;
-  //         assert |transferredContents.Keys| == |transferredContents|;
-  //         assert |Contents.Keys| == |Contents|;
-  //         assert |transferredContents| <= |Contents|;
-  //         assert newUnderlying.Count as nat < newUnderlying.Storage.Length - 1;
-  //         // -- mutation --
-  //         ghost var _ := newUnderlying.Insert(item.key, item.value);
-  //         transferredContents := transferredContents[item.key := item.value];
-  //         // --------------
-
-  //         forall key | key in newUnderlying.Contents
-  //         ensures exists slot: Slot :: (
-  //             && slot.slot < i as nat + 1
-  //             && ValidSlot(Underlying.Storage.Length, slot)
-  //             && Underlying.Storage[slot.slot].Entry?
-  //             && Underlying.Storage[slot.slot].key == key)
-  //         {
-  //           if key == item.key {
-  //             assert ValidSlot(Underlying.Storage.Length, Slot(i as nat));
-  //             assert exists slot: Slot :: (
-  //                 && slot.slot < i as nat + 1
-  //                 && ValidSlot(Underlying.Storage.Length, slot)
-  //                 && Underlying.Storage[slot.slot].Entry?
-  //                 && Underlying.Storage[slot.slot].key == key);
-  //           } else {
-  //             assert exists slot: Slot :: (
-  //                 && slot.slot < i as nat + 1
-  //                 && ValidSlot(Underlying.Storage.Length, slot)
-  //                 && Underlying.Storage[slot.slot].Entry?
-  //                 && Underlying.Storage[slot.slot].key == key);
-  //           }
-  //         }
-  //         assert |transferredContents| == newUnderlying.Count as nat;
-  //         assert MapFromStorage(Underlying.Storage[..i+1]) == transferredContents;
-  //       } else {
-  //         assert forall key :: key in newUnderlying.Contents ==> exists slot: Slot :: (
-  //             && slot.slot < i as nat
-  //             && ValidSlot(Underlying.Storage.Length, slot)
-  //             && Underlying.Storage[slot.slot].Entry?
-  //             && Underlying.Storage[slot.slot].key == key);
-  //         assert |transferredContents| <= newUnderlying.Count as nat;
-  //         assert MapFromStorage(Underlying.Storage[..i+1]) == transferredContents;
-  //       }
-
-  //       // -- increment --
-  //       i := i + 1;
-  //       // ---------------
-
-  //       assert MapFromStorage(Underlying.Storage[..i]) == transferredContents;
-  //     }
-
-  //     assert i as nat == Underlying.Storage.Length;
-  //     assert Underlying.Storage[..i] == Underlying.Storage[..];
-
-  //     assert MapFromStorage(Underlying.Storage[..]) == transferredContents;
-  //     UnderlyingInvImpliesMapFromStorageMatchesContents(newUnderlying, transferredContents);
-  //     assert transferredContents == Contents;
-
-  //     assert |Contents| == Count as nat;
-
-  //     assert forall key :: key in Contents ==> key in newUnderlying.Contents && newUnderlying.Contents[key] == Some(Contents[key]);
-  //     assert forall key :: key !in Contents ==> key !in newUnderlying.Contents || newUnderlying.Contents[key].None?;
-
-  //     assert newUnderlying.Inv();
-  //     assert UnderlyingInv(newUnderlying);
-  //     assert UnderlyingContentsMatchesContents(newUnderlying, Contents);
-  //     assert MapFromStorage(newUnderlying.Storage[..]) == Contents;
-  //     assert newUnderlying.Count as nat < newUnderlying.Storage.Length - 2;
-
-  //     assert fresh(newUnderlying);
-  //     assert fresh(newUnderlying.Storage);
-
-  //     // -- mutation --
-  //     Underlying := newUnderlying;
-  //     // --------------
-
-  //     assert fresh(Underlying);
-  //     assert fresh(Underlying.Storage);
-  //     Repr := { this, Underlying } + Underlying.Repr;
-  //     assert Underlying.Repr == { Underlying, Underlying.Storage };
-  //     assert Repr == { this, Underlying, Underlying.Storage };
-  //     assert forall r :: r in Repr ==> r in old(Repr) || fresh(r);
-
-  //     assert Underlying.Count as nat < Underlying.Storage.Length - 2;
-  //     assert Contents == old(Contents);
-  //     assert Count == old(Count);
-  //     assert Count <= Underlying.Count;
-  //     assert Inv();
-  //   }
+      MutableMapModel.LemmaReallocResult(old(I()));
+    }
 
   //   method Insert(key: uint64, value: V) returns (replaced: Option<V>)
   //     requires Inv()
